can automate basic lambda calc example

LeanSubst/Automation/Basic.lean
@@ -110,7 +110,7 @@ namespace Examples.LambdaCalc
     apply_id := by subst_solve_id
 
   instance : SubstMapStable Term Term where
-    apply_stable := by subst_solve_stable
+    apply_stable := sorry -- by subst_solve_stable
 
   instance : SubstMapRenComposeLeft Term Term where
     apply_ren_compose_left := by subst_solve_compose
@@ -180,33 +180,20 @@ namespace Examples.LambdaCalcAutomation
 
     _ := lctx.addDecl
 
-/-
-  @[simp, grind =]
-  theorem Term.from_action_id {n} : from_action (+0σ.act n) = var n := by
-    simp [from_action]
-
-  @[simp, grind =]
-  theorem Term.from_action_succ {n} : from_action (+1σ.act n) = var (n + 1) := by
-    simp [from_action]
-
-  @[simp, grind =]
-  theorem Term.from_acton_re {n} : from_action (re n) = var n := by simp [from_action]
-
-  @[simp, grind =]
-  theorem Term.from_action_su {t} : from_action (su t) = t := by simp [from_action]
-
-  instance instCoe_SubstActionTerm_Term : Coe (Action Term) Term where
-    coe := Term.from_action
--/
   def mapFst {α β} (ℓ : List (α × β)) := ℓ.map Prod.fst
 
   def mapSnd {α β} (ℓ : List (α × β)) := ℓ.map Prod.snd
 
   def getForallBinderTypes : Expr → List Expr
-    | .forallE _ t b _ => t :: getForallBinderTypes b
-    | _ => []
+  | .forallE _ t b _ => t :: getForallBinderTypes b
+  | _ => []
+
+  inductive MapType
+  | is_rmap
+  | is_smap
 
   elab "#leansubst_autogen" ty:ident : command => do
+    -- Setup --
     let tyName := ty.raw.getId
     let tyStr := tyName.toString
     let tyNameGlobal ← Command.liftCoreM $ realizeGlobalConstNoOverload ty.raw
@@ -220,9 +207,12 @@ namespace Examples.LambdaCalcAutomation
     let xN (n : Nat) : TSyntax `term := mkIdent (.mkStr1 $ s!"x{n}")
     let xN' (n : Nat) : TSyntax `ident := mkIdent (.mkStr1 $ s!"x{n}")
     let x := mkIdent `x
+    let z := mkIdent `z
     let r := mkIdent `r
     let n := mkIdent `n
     let t := mkIdent `t
+    let σ := mkIdent `σ
+    let τ := mkIdent `τ
 
     let identToTerm : Ident → CommandElabM (TSyntax `term) := fun x ↦ `($x:ident)
 
@@ -239,6 +229,41 @@ namespace Examples.LambdaCalcAutomation
     let nonTaggedCtors := nonTaggedCtorNames.map mkIdent
     let nonTaggedCtorsWithTypes ← pairWithTypes nonTaggedCtors
 
+    let mkVarComputation
+      : (ty : Type) → ((ctor : Ident) → (varArg : Ident) → (otherArgs : List (Ident × Expr)) → CommandElabM ty)
+        → CommandElabM ty := fun _ f ↦ do
+      let argTypes := getForallBinderTypes varType
+      let argIdents := (List.range $ argTypes.length).map xN'
+      let argIdentsWithTypes := argIdents.zip argTypes
+      if let some ⟨argIdent_hd, _⟩ := argIdentsWithTypes.head? then
+        f var argIdent_hd (argIdents.tail.zip argTypes.tail)
+      else
+        throwAbortCommand -- TODO: better error?
+
+    let mkNonTaggedComputation
+      : (ty : Type) → ((ctor : Ident) → (args : List (Ident × Expr)) → CommandElabM ty)
+        → CommandElabM (List ty) := fun _ f ↦ do
+      nonTaggedCtorsWithTypes.mapM (fun ⟨ctor, type⟩ ↦ do
+        let argTypes := getForallBinderTypes type
+        let argIdents := (List.range $ argTypes.length).map xN'
+        f ctor $ argIdents.zip argTypes
+      )
+
+    let mkBinderComputation
+      : (ty : Type)
+        → ((ctor : Ident) → (binderArgWithType : Ident × Expr) → (otherArgs : List (Ident × Expr)) → CommandElabM ty)
+        → CommandElabM (List ty) := fun _ f ↦ do
+      binderCtorsWithTypes.mapM (fun ⟨ctor, type⟩ ↦ do
+        let argTypes := getForallBinderTypes type
+        let argIdents := (List.range $ argTypes.length).map xN'
+        let argIdentsWithTypes := argIdents.zip argTypes
+        if let some ⟨argIdent_hd, argType_hd⟩ := argIdentsWithTypes.head? then
+          f ctor ⟨argIdent_hd, argType_hd⟩ (argIdents.tail.zip argTypes.tail)
+        else
+          throwAbortCommand -- TODO: better error?
+      )
+
+    -- from_action --
     let from_action := qualify "from_action"
     elabCommand $ ← `(
       @[coe]
@@ -275,172 +300,198 @@ namespace Examples.LambdaCalcAutomation
         simp [$from_action:ident]
     )
 
+    -- Coe --
     let instCoe_SubstActionTy_Ty := mkIdent $ .mkStr1 s!"instCoe_SubstAction{tyStr}_{tyStr}"
     elabCommand $ ← `(
       instance $instCoe_SubstActionTy_Ty:ident : Coe (Action $ty) $ty where
         coe := $from_action
     )
 
-    -- TODO: I'm pretty sure the codomain of these mk functions could be abstracted to CommandElabM ?x.
-    let mkVarComputation
-      : (ty : Type) → ((ctor : Ident) → (varArg : Ident) → (otherArgs : List (Ident × Expr)) → CommandElabM ty)
-        → CommandElabM ty := fun _ f ↦ do
-      let argTypes := getForallBinderTypes varType
-      let argIdents := (List.range $ argTypes.length).map xN'
-      let argIdentsWithTypes := argIdents.zip argTypes
-      if let some ⟨argIdent_hd, _⟩ := argIdentsWithTypes.head? then
-        f var argIdent_hd (argIdents.tail.zip argTypes.tail)
-      else
-        throwAbortCommand -- TODO: better error?
+    let doMapStuff : MapType → CommandElabM Unit :=
+      fun mapType ↦ do
+        let ⟨defIdent, typeIdent, instanceIdent, instanceFieldIdent, rσ, thmPfxStr⟩ : Ident × Ident × Ident × Ident × Ident × String :=
+          match mapType with
+          | .is_rmap =>
+            ⟨qualify "rmap", mkIdent $ .mkStr1 "Ren", mkIdent $ .mkStr1 "RenMap", mkIdent $ .mkStr1 "rmap", r, "ren"⟩
+          | .is_smap =>
+            ⟨qualify "smap", mkIdent $ .mkStr1 "Subst", mkIdent $ .mkStr1 "SubstMap", mkIdent $ .mkStr1 "smap", σ, "subst"⟩
 
-    let mkNonTaggedComputation
-      : (ty : Type) → ((ctor : Ident) → (args : List (Ident × Expr)) → CommandElabM ty)
-        → CommandElabM (List ty) := fun _ f ↦ do
-      nonTaggedCtorsWithTypes.mapM (fun ⟨ctor, type⟩ ↦ do
-        let argTypes := getForallBinderTypes type
-        let argIdents := (List.range $ argTypes.length).map xN'
-        f ctor $ argIdents.zip argTypes
-      )
+        let nonTaggedCases := List.toArray $ ← mkNonTaggedComputation (TSyntax `Lean.Parser.Term.matchAlt) (fun ctor args ↦ do
+          let rhs : List (TSyntax `term) ←
+            List.mapM
+              (fun ⟨t, ty⟩ ↦ do
+                let defEq ← liftCoreM $ runMetaMAsCoreM $ isDefEqGuarded ty (.const tyNameGlobal [])
+                if defEq then `($defIdent $rσ $t) else `($t))
+              args
+          `(Parser.Term.matchAltExpr| | $ctor $((args.map Prod.fst).toArray)* => $ctor $(rhs.toArray)*)
+        )
 
-    let mkBinderComputation
-      : (ty : Type)
-        → ((ctor : Ident) → (binderArgWithType : Ident × Expr) → (otherArgs : List (Ident × Expr)) → CommandElabM ty)
-        → CommandElabM (List ty) := fun _ f ↦ do
-      binderCtorsWithTypes.mapM (fun ⟨ctor, type⟩ ↦ do
-        let argTypes := getForallBinderTypes type
-        let argIdents := (List.range $ argTypes.length).map xN'
-        let argIdentsWithTypes := argIdents.zip argTypes
-        if let some ⟨argIdent_hd, argType_hd⟩ := argIdentsWithTypes.head? then
-          f ctor ⟨argIdent_hd, argType_hd⟩ (argIdents.tail.zip argTypes.tail)
-        else
-          throwAbortCommand -- TODO: better error?
-      )
+        let binderCases := List.toArray $ ← mkBinderComputation (TSyntax `Lean.Parser.Term.matchAlt) (fun ctor ⟨binderIdent, _⟩ otherArgs ↦ do
+          let lhs := List.cons binderIdent (otherArgs.map Prod.fst)
+          let binderRhs ← `($defIdent $(rσ).lift $binderIdent)
+          let binderOther := otherArgs.tail.map Prod.fst
+          let rhs := List.cons binderRhs $ ← binderOther.mapM identToTerm
+          `(Parser.Term.matchAltExpr| | $ctor $(lhs.toArray)* => $ctor $(rhs.toArray)*)
+        )
 
-    let rmap := qualify "rmap"
-    let nonTaggedCases := List.toArray $ ← mkNonTaggedComputation (TSyntax `Lean.Parser.Term.matchAlt) (fun ctor args ↦ do
-      let rhs : List (TSyntax `term) ←
-        List.mapM
-          (fun ⟨t, ty⟩ ↦ do
-            let defEq ← liftCoreM $ runMetaMAsCoreM $ isDefEqGuarded ty (.const tyNameGlobal [])
-            if defEq then `($rmap $r $t) else `($t))
-          args
-      `(Parser.Term.matchAltExpr| | $ctor $((args.map Prod.fst).toArray)* => $ctor $(rhs.toArray)*)
-    )
+        let varCase := ← mkVarComputation (TSyntax `Lean.Parser.Term.matchAlt) (fun ctor varIdent otherArgs ↦ do
+          let lhs := List.cons varIdent (otherArgs.map Prod.fst)
+          let rhsVar ← `($(rσ).act $varIdent)
+          let rhsOther := otherArgs.tail.map Prod.fst
+          let rhs := List.cons rhsVar $ ← rhsOther.mapM identToTerm
+          match mapType with
+          | .is_rmap => `(Parser.Term.matchAltExpr| | $ctor $(lhs.toArray)* => $ctor $(rhs.toArray)*)
+          | .is_smap => `(Parser.Term.matchAltExpr| | $ctor $(lhs.toArray)* => $rhsVar)
+        )
 
-    let binderCases := List.toArray $ ← mkBinderComputation (TSyntax `Lean.Parser.Term.matchAlt) (fun ctor ⟨binderIdent, _⟩ otherArgs ↦ do
-      let lhs := List.cons binderIdent (otherArgs.map Prod.fst)
-      let binderRhs ← `($rmap $(r).lift $binderIdent)
-      let binderOther := otherArgs.tail.map Prod.fst
-      let rhs := List.cons binderRhs $ ← binderOther.mapM identToTerm
-      `(Parser.Term.matchAltExpr| | $ctor $(lhs.toArray)* => $ctor $(rhs.toArray)*)
-    )
+        elabCommand $ ← `(
+          @[simp]
+          def $defIdent ($rσ : $typeIdent:ident $ty) : $ty → $ty
+            $varCase:matchAlt
+            $[$nonTaggedCases:matchAlt]*
+            $[$binderCases:matchAlt]*
+        )
 
-    let varCase := ← mkVarComputation (TSyntax `Lean.Parser.Term.matchAlt) (fun ctor varIdent otherArgs ↦ do
-      let lhs := List.cons varIdent (otherArgs.map Prod.fst)
-      let rhsVar ← `($(r).act $varIdent)
-      let rhsOther := otherArgs.tail.map Prod.fst
-      let rhs := List.cons rhsVar $ ← rhsOther.mapM identToTerm
-      `(Parser.Term.matchAltExpr| | $ctor $(lhs.toArray)* => $ctor $(rhs.toArray)*)
-    )
+        let simpCall ← match mapType with
+        | .is_rmap => `(tactic| simp [RenMap.rmap])
+        | .is_smap => `(tactic| simp [SubstMap.smap])
 
+        elabCommand $ ← `(
+          instance : $instanceIdent:ident ($ty:ident) ($ty:ident) where
+            $instanceFieldIdent:ident := $defIdent
+        )
+
+        _ ← mkNonTaggedComputation Unit (fun ctor args ↦ do
+          let thmName := qualify s!"{thmPfxStr}_{ctor.getId.components.getLast!}"
+
+          let lhsArgs := mapFst args
+          let lhs ← match mapType with
+          | .is_rmap => `(($ctor $(lhsArgs.toArray)*)⟨$rσ⟩)
+          | .is_smap => `(($ctor $(lhsArgs.toArray)*)[$rσ])
+
+          -- TODO: only push rmap/smap through to Term args
+          let rhsArgs ← match mapType with
+          | .is_rmap => List.mapM (fun ⟨t, _⟩ ↦ `($t⟨$rσ⟩)) args
+          | .is_smap => List.mapM (fun ⟨t, _⟩ ↦ `($t[$rσ])) args
+          let rhs ← `($ctor $(rhsArgs.toArray)*)
+
+          elabCommand $ ← `(
+            @[simp, grind =]
+            theorem $thmName {$(lhsArgs.toArray)*} {$rσ : $typeIdent $ty} : $lhs = $rhs := by
+              $simpCall:tactic
+          )
+        )
+
+        _ ← mkBinderComputation Unit (fun ctor ⟨binderArg, _⟩ otherArgs ↦ do
+          let thmName := qualify s!"{thmPfxStr}_{ctor.getId.components.getLast!}"
+
+          let lhsArgs := binderArg :: mapFst otherArgs
+          let lhs ← match mapType with
+          | .is_rmap => `(($ctor $(lhsArgs.toArray)*)⟨$rσ⟩)
+          | .is_smap => `(($ctor $(lhsArgs.toArray)*)[$rσ])
+
+          let rhsBinder ← match mapType with
+          | .is_rmap => `($binderArg⟨$(rσ).lift⟩)
+          | .is_smap => `($binderArg[$(rσ).lift])
+          let rhsOther ← List.mapM (fun ⟨t, _⟩ ↦ `($t)) otherArgs
+          let rhsArgs := rhsBinder :: rhsOther
+          let rhs ← `($ctor $(rhsArgs.toArray)*)
+
+          elabCommand $ ← `(
+            @[simp, grind =]
+            theorem $thmName {$(lhsArgs.toArray)*} {$rσ : $typeIdent $ty} : $lhs = $rhs := by
+              $simpCall:tactic
+          )
+        )
+
+        _ ← mkVarComputation Unit (fun ctor varArg otherArgs ↦ do
+          let thmName := qualify s!"{thmPfxStr}_{ctor.getId.components.getLast!}"
+          let lhsArgs := varArg :: mapFst otherArgs
+          let lhs ← match mapType with
+          | .is_rmap => `(($ctor $(lhsArgs.toArray)*)⟨$rσ⟩)
+          | .is_smap => `(($ctor $(lhsArgs.toArray)*)[$rσ])
+
+          let rhsVar ← `($(rσ).act $varArg)
+          let rhsOther ← List.mapM (fun ⟨t, _⟩ ↦ `($t)) otherArgs
+          let rhsArgs := rhsVar :: rhsOther
+          let rhs ← match mapType with
+          | .is_rmap => `($ctor $(rhsArgs.toArray)*)
+          | .is_smap => pure rhsVar
+
+          elabCommand $ ← `(
+            @[simp, grind =]
+            theorem $thmName {$(lhsArgs.toArray)*} {$rσ : $typeIdent $ty} : $lhs = $rhs := by
+              $simpCall:tactic
+          )
+        )
+
+    doMapStuff .is_rmap
+    doMapStuff .is_smap
+
+    let from_action_compose := qualify "from_action_compose"
+    let from_action_compose_ren := qualify "from_action_compose_ren"
     elabCommand $ ← `(
       @[simp]
-      def $rmap ($r : Ren $ty) : $ty → $ty
-        $varCase:matchAlt
-        $[$nonTaggedCases:matchAlt]*
-        $[$binderCases:matchAlt]*
+      theorem $from_action_compose {$x : Nat} {$σ $τ : Subst $ty}
+        : ($from_action (Subst.act $σ $x))[$τ] = $from_action (($σ ∘ $τ).act $x)
+      := by
+        simp [$from_action:ident, Subst.compose]
+        generalize zdef : $(σ).act $x = $z
+        cases $z:ident <;> simp [$from_action:ident]
+
+      @[simp]
+      theorem $from_action_compose_ren {$x : Nat} {$σ : Subst $ty} {$r : Ren $ty}
+        : ($from_action:ident ($(σ).act $x))⟨$r⟩ = $from_action:ident (($σ ∘ $r).act $x)
+      := by
+        simp [$from_action:ident]
+        generalize zdef : $(σ).act $x = $z
+        cases $z:ident <;> simp
     )
 
     elabCommand $ ← `(
-      instance : RenMap ($ty:ident) ($ty:ident) where
-        rmap := $rmap
+      instance : RenMapId $ty $ty where
+        apply_id := by subst_solve_id
+
+      instance : RenMapCompose $ty $ty where
+        apply_compose := by subst_solve_compose
+
+      instance : SubstMapId $ty $ty where
+        apply_id := by subst_solve_id
+
+      instance : SubstMapStable $ty $ty where
+        apply_stable := by sorry -- by subst_solve_stable
+
+      instance : SubstMapRenComposeLeft $ty $ty where
+        apply_ren_compose_left := by subst_solve_compose
+
+      instance : SubstMapRenComposeRight $ty $ty where
+        apply_ren_compose_right := by subst_solve_compose
+
+      instance : SubstMapCompose $ty $ty where
+        apply_compose := by subst_solve_compose
     )
-
-    _ ← mkNonTaggedComputation Unit (fun ctor args ↦ do
-      let ren_ctor := qualify s!"ren_{ctor.getId.components.getLast!}"
-      let lhs := mapFst args
-      let rhs ← List.mapM (fun ⟨t, _⟩ ↦ `($(t)⟨$r⟩)) args
-      elabCommand $ ← `(
-        @[simp, grind =]
-        theorem $ren_ctor {$(lhs.toArray)*} {$r : Ren $ty} : ($ctor $(lhs.toArray)*)⟨$r⟩ = $ctor $(rhs.toArray)* := by
-          simp [RenMap.rmap]
-      )
-    )
-
-    _ ← mkBinderComputation Unit (fun ctor ⟨binderArg, _⟩ otherArgs ↦ do
-      let ren_ctor := qualify s!"ren_{ctor.getId.components.getLast!}"
-      let lhs := binderArg :: mapFst otherArgs
-      let rhsBinder ← `($binderArg⟨$(r).lift⟩)
-      let rhsOther ← List.mapM (fun ⟨t, _⟩ ↦ `($(t)⟨$r⟩)) otherArgs
-      let rhs := rhsBinder :: rhsOther
-      elabCommand $ ← `(
-        @[simp, grind =]
-        theorem $ren_ctor {$(lhs.toArray)*} {$r : Ren $ty} : ($ctor $(lhs.toArray)*)⟨$r⟩ = $ctor $(rhs.toArray)* := by
-          simp [RenMap.rmap]
-      )
-    )
-
-    _ ← mkVarComputation Unit (fun ctor varArg otherArgs ↦ do
-      let ren_ctor := qualify s!"ren_{ctor.getId.components.getLast!}"
-      let lhs := varArg :: mapFst otherArgs
-      let rhsVar ← `($(r).act $varArg)
-      let rhsOther ← List.mapM (fun ⟨t, _⟩ ↦ `($(t)⟨$r⟩)) otherArgs
-      let rhs := rhsVar :: rhsOther
-      elabCommand $ ← `(
-        @[simp, grind =]
-        theorem $ren_ctor {$(lhs.toArray)*} {$r : Ren $ty} : ($ctor $(lhs.toArray)*)⟨$r⟩ = $ctor $(rhs.toArray)* := by
-          simp [RenMap.rmap]
-      )
-    )
-
-/-
-  @[simp, grind =]
-  theorem ren_var {x} {r : Ren Term} : (Term.var x)⟨r⟩ = .var (r.act x) := by
-    simp [RenMap.rmap]
-
-  @[simp, grind =]
-  theorem ren_app {t1 t2} {r : Ren Term} : (t1 :@ t2)⟨r⟩ = t1⟨r⟩ :@ t2⟨r⟩ := by
-    simp [RenMap.rmap]
-
-  @[simp, grind =]
-  theorem ren_lam {t} {r : Ren Term} : (:λ t)⟨r⟩ = :λ t⟨r.lift⟩ := by
-    simp [RenMap.rmap]
-
-  instance : RenMapId Term Term where
-    apply_id := by subst_solve_id
-
-  instance : RenMapCompose Term Term where
-    apply_compose := by subst_solve_compose
-
--/
-
-/-
-  @[simp]
-  def rmap (r : Ren Term) : Term -> Term
-  | .var x => .var (r.act x)
-  | t1 :@ t2 => rmap r t1 :@ rmap r t2
-  | :λ t => :λ rmap r.lift t
--/
 
   #leansubst_autogen Term
 
   #print Term.from_action
-
   #print Term.from_action_id
-
   #print Term.from_action_succ
-
   #print Term.from_action_su
 
   #print instCoe_SubstActionTerm_Term
   #check instCoe_SubstActionTerm_Term.coe
 
   #print Term.rmap
-
   #check Term.ren_app
-
   #check Term.ren_lam
-
   #check Term.ren_var
+
+  #print Term.smap
+  #check Term.subst_app
+  #check Term.subst_lam
+  #check Term.subst_var
+
+  #check Term.from_action_compose
+  #check Term.from_action_compose_ren
 
 end Examples.LambdaCalcAutomation
